shake + writing on binary trees

Shake.hs
@@ -1,0 +1,45 @@
+#!/usr/bin/env stack
+-- stack --resolver lts-11.3 script --package shake
+
+import Development.Shake
+import Development.Shake.Command
+import Development.Shake.FilePath
+import Development.Shake.Util
+
+-- pdf file extension
+pdf :: FilePath
+pdf = "pdf"
+
+-- lagda file extension
+lagda :: FilePath
+lagda = "lagda"
+
+-- tex file extension
+tex :: FilePath
+tex = "tex"
+
+-- lagda modules used to build the thesis
+thesis_lagda_modules :: [String]
+thesis_lagda_modules = [ "main" , "tree" ]
+
+main :: IO ()
+main = shakeArgs shakeOptions $ do
+  want ["thesis/main" <.> pdf]
+
+  phony "distclean" $ do
+    putNormal "Cleaning files in thesis"
+    cmd_ "latexmk -c -cd thesis/main.tex"
+    removeFilesAfter "thesis" ["*.tex", "*.bbl"]
+
+  "thesis/*.tex" %> \out -> do
+    let inp = out -<.> lagda
+    need [inp]
+    cmd_ (Cwd "thesis") "lhs2TeX --agda -o" [takeFileName out] (takeFileName inp)
+
+  "thesis/main" <.> pdf %> \out -> do
+    let mods = [ "thesis" </> f <.> tex | f <- thesis_lagda_modules]
+        bib  = "thesis/main.bib"
+        fmt  = "thesis/thesis.fmt"
+        sty  = "thesis/agda.sty"
+    need (bib : fmt : sty : mods)
+    cmd_ "latexmk -pdf -cd -xelatex thesis/main.tex"
