src/Thesis/Fold.v
@@ -8,6 +8,7 @@ Fixpoint eval (t : Tree) : nat :=
     | Tip x => x
     | Node t1 t2 => eval t1 + eval t2
   end.
+
     
 (* dummy wrapper to lift Tree to Prop *)
 Inductive TreeP : Prop :=
@@ -19,14 +20,9 @@ Fixpoint LiftTree (t : Tree) : TreeP :=
     | Tip x => TreeP_Tip x
     | Node t1 t2 => TreeP_Node (LiftTree t1) (LiftTree t2)
   end.
-Definition Stack : Type := list (Tree + (TreeP * nat)).
-Definition Zipper : Type := Tree * Stack.
 
-Fixpoint to_left (t : Tree) (s : Stack) : Zipper :=
-  match t with
-    | Node t1 t2 => to_left t1 (cons (inl t2) s)
-    | Tip x      => (Tip x , s)
-  end.
+Definition Stack : Type := list (Tree + (TreeP * nat)).
+Definition Zipper : Type := nat * Stack.
 
 (* plug_up lives in Prop because uses the TreeP from the Stack *)  
 Fixpoint plug_up (t : TreeP) (s : Stack) : TreeP :=
@@ -36,71 +32,46 @@ Fixpoint plug_up (t : TreeP) (s : Stack) : TreeP :=
     | cons (inr (t1 , _)) s => plug_up (TreeP_Node t1 t) s
   end.
 
-Definition plug_up_zipper (z : Zipper) : TreeP :=
-  plug_up (LiftTree (fst z)) (snd z).
-
-Lemma to_left_preserves_plug_up : 
-  forall t s t' s', to_left t s = (t' , s') -> plug_up (LiftTree t) s = plug_up (LiftTree t') s'.
-Proof.
-  intro.
-  induction t.
-    + intros. inversion H. reflexivity.
-    + intros. simpl in H. apply IHt1 in H. simpl in H. assumption.
-Qed.
-
-(* the (t : TreeP) is only hold to reconstruct the full Tree *)
-Fixpoint to_up_right (t : TreeP) (n : nat) (s : Stack) : Zipper + nat :=
-  match  s with
-    | nil                   => inr n
-    | cons (inl t1) s       => inl (t1 , cons (inr (t , n)) s)
-    | cons (inr (t1 , m)) s => to_up_right (TreeP_Node t1 t) (n + m) s
-  end.
-
-Lemma to_up_right_preservers_plug_up : 
-  forall t s t' s' n , to_up_right t n s = inl (t' , s') 
-    -> plug_up t s = plug_up (LiftTree t') s'.
-Proof.
-  intros t s.
-  generalize dependent t.
-  induction s.
-    + intros. inversion H.
-    + intros. destruct a.
-      * inversion H. simpl. reflexivity.
-      * destruct p. inversion H. apply IHs in H1. simpl. assumption.
-Qed.
-
-Definition right (z : Zipper) : Zipper + nat :=
-  match z with
-    | (Tip x , s)      => to_up_right (TreeP_Tip x) x s
-    | (Node t1 t2 , s) => inl (to_left (Node t1 t2) s)
-  end.
- 
-Lemma right_preserves_plug_up :
- forall t s t' s', right (t , s) = inl (t' , s') 
-    -> plug_up (LiftTree t) s = plug_up (LiftTree t') s'.
-Proof.
-  intros.
-  destruct t.
-    + simpl. apply (to_up_right_preservers_plug_up _ _ _ _ n). assumption.
-    + apply (to_left_preserves_plug_up). inversion H. simpl. reflexivity.
-Qed.
 
 (* A Prop version of the Zipper *)
 Inductive ZipperP : Prop := 
-  | ZipperP_constr : TreeP * Stack -> ZipperP.
+  | ZipperP_constr : nat * Stack -> ZipperP.
 
 Definition LiftZipper (z : Zipper) : ZipperP :=
-  ZipperP_constr (LiftTree (fst z) , snd z).
+  ZipperP_constr (fst z , snd z).
+
+Definition plug_up_zipper (z : ZipperP) : TreeP :=
+  match z with
+    | ZipperP_constr (n , s) => plug_up (TreeP_Tip n) s
+  end.
+
+
+Fixpoint to_left (t : Tree) (s : Stack) : Zipper + nat :=
+  match t with
+    | Node t1 t2 => to_left t1 (cons (inl t2) s)
+    | Tip x      => inl (x , s)
+  end.
+
+Fixpoint to_up_right (t : TreeP) (n : nat) (s : Stack) : Zipper + nat :=
+  match  s with
+    | nil                   => inr n
+    | cons (inl t1) s       => to_left t1 s
+    | cons (inr (t1 , m)) s => to_up_right (TreeP_Node t1 t) (n + m) s
+  end.
+
+Definition step (z : Zipper) : Zipper + nat :=
+  to_up_right (TreeP_Tip (fst z)) (fst z) (snd z).
+
+
+
+
+
 
 Inductive Smaller_than : ZipperP -> ZipperP -> Prop :=
-  | Right_Left : forall n t t1 t2 s1 s2, plug_up t1 s1 = (LiftTree t) ->
-                   Smaller_than (ZipperP_constr (t1 , cons (inr (plug_up t2 s2 , n)) s1))
-                                (ZipperP_constr (t2 , cons (inl t) s2))
-
   | Right_Step : forall n t t1 t2 s1 s2, 
                    Smaller_than (ZipperP_constr (t1 , s1)) 
                                 (ZipperP_constr (t2 , s2)) 
-                   -> 
+                   ->     
                    Smaller_than (ZipperP_constr (t1 , cons (inr (t , n)) s1))
                                 (ZipperP_constr (t2 , cons (inr (t , n)) s2))
 
@@ -109,13 +80,59 @@ Inductive Smaller_than : ZipperP -> ZipperP -> Prop :=
                                 (ZipperP_constr (t2 , s2)) -> 
                    Smaller_than (ZipperP_constr (t1 , cons (inl t) s1)) 
                                 (ZipperP_constr (t2 , cons (inl t) s2))
-  | Right_base : forall t t1 s n, 
-                   Smaller_than (ZipperP_constr (t1 , cons (inr (t , n)) s))
-                                (ZipperP_constr (TreeP_Node t1 (plug_up t s) , nil)).
-                                
-                                
-Notation "x < y" := (Smaller_than x y).
 
+ | Right_Left : forall n t t1 t2 s1 s2, plug_up (TreeP_Tip t1) s1 = (LiftTree t) ->
+         Smaller_than (ZipperP_constr (t1 , cons (inr (plug_up (TreeP_Tip t2) s2 , n)) s1))
+                      (ZipperP_constr (t2 , cons (inl t) s2)).
+
+
+
+
+
+
+
+
+
+Inductive Smaller_than_ix (t : TreeP) : ZipperP -> ZipperP -> Prop :=
+  lt : forall z1 z2, plug_up_zipper z1 = t -> plug_up_zipper z2 = t -> Smaller_than z1 z2 -> 
+     Smaller_than_ix t z1 z2.
+     
+Notation "x < y" := (Smaller_than x y).
+Notation "[ t ] x < y" := (Smaller_than_ix t x y) (at level 50).
+(*
+      accR : ∀ {l r : Tree} (t : ℕ) (s : Stack) eq₁
+               {a : A} {eq : treeCata tAlg l ≡ a} →
+               Acc ([[_]]⇓_<_ r) ((t , s) ,, Node-injᵣ eq₁) → 
+             (y : Zipper⇓ (Node l r)) → [[ Node l r ]]⇓ y < ((t , inj₂ (a , l , eq) ∷ s) ,, eq₁) → Acc ([[_]]⇓_<_ (Node l r)) y
+      accR t s eq₁ {a} {eq} (acc rs) .((t₁ , inj₂ (a , _ , eq) ∷ s₁) ,, refl) (<-Right-Step {t₁ = t₁} {s₁ = s₁} refl .eq₁ p)
+          = acc (accR t₁ s₁ refl (rs ((t₁ , s₁) ,, refl) p))
+*)
+Lemma accR : forall l r t s n, Acc (Smaller_than_ix r) (ZipperP_constr (t , s)) 
+           -> forall y, Smaller_than_ix (TreeP_Node l r) y 
+                                        (ZipperP_constr (t , cons (inr (l , n)) s)) 
+           -> Acc (Smaller_than_ix (TreeP_Node l r)) y.
+Proof.
+  intros l r t s n.
+  intros ACC_TS y.
+  intro SMALLER_Y.
+  destruct SMALLER_Y.
+  destruct H1.
+
+Theorem Smaller_than_ix_acc : forall t, forall z, Acc (Smaller_than_ix t) z.
+Proof.
+  intros.
+  rename z into x.
+  constructor.
+  intro.
+  intro Y_LT_Z.
+  
+  destruct Y_LT_Z as [y x].
+  destruct H1. (*as [ xt  | y | y ].*)
+  - (* Both to the right *)
+    Acc_ind
+  - admit.
+  - admit.
+  
 Lemma Smaller_than_acc : forall z, Acc Smaller_than z.
 Proof.
   intros. destruct z. destruct p. induction s.
