thesis/tree.lagda
@@ -1,0 +1,673 @@
+%include polycode.fmt
+%include thesis.fmt
+
+%{
+%format Tree  = "\AD{Tree}"
+%format Tip   = "\AI{Tip}"
+%format Node  = "\AI{Node}"
+%format eval  = "\AF{eval}"
+%format +     = "\AF{+}"
+%format pretty   = "\AF{pretty}"
+%format TreeAlg  = "\AD{TreeAlg}"
+%format A        = "\AB{A}"
+%format NodeA    = "\AB{NodeA}"
+%format TipA     = "\AB{TipA}"
+%format treeCata = "\AF{treeCata}"
+
+%format UZipper = "\AD{UZipper}"
+%format Stack = "\AD{Stack}"
+%format Top   = "\AD{Top}"
+%format Left  = "\AD{Left}"
+%format Right = "\AD{Right}"
+%format load  = "\AF{load}"
+%format unload  = "\AF{unload}"
+%format foldr = "\AF{foldr}"
+%format foldl = "\AF{foldl}"
+
+%format plugD   = "\AF{plug\ensuremath{\!\!\Downarrow}}"
+%format plugZD  = "\AF{plugZ\ensuremath{\!\!\Downarrow}}"
+%format ZipperD = "\AD{Zipper\ensuremath{\!\!\Downarrow}}"
+%format forgetD = "\AF{forget\ensuremath{\!\!\Downarrow}}"
+
+%format step = "\AF{step}"
+
+%format plugU = "\AF{plug\ensuremath{\!\!\Uparrow}}"
+%format plusOp = "\AF{\_+\_}"
+
+
+\section{Verified tail-recursive fold for binary trees}\label{sec:tree}
+
+  In this chapter, we present the transformation of a catamorphism for binary
+  trees with natural numbers in the leaves onto a tail-recursive function.
+  Moreover, we show how to prove that the resulting function terminates and that
+  it is correct (for every possible input it computes the same result as the
+  original fold).
+
+  In order to do so, in \cref{subsec:bintree} we introduce the type of binary
+  trees along with several examples of evaluation functions and how their common
+  structure can be abstracted into a catamorphism. Then, in \cref{subsec:zipper},
+  we explain the concept of a Zipper with its many type indexed variants and in
+  \cref{subsec:onestep}.
+
+  % In order to do, we first introduce the type of binary trees. In \subi We
+  % provide both a proof of the termination of the transformation by defining a
+  % suitable well-founded relation and also prove that the transformation is
+  % correct.
+
+
+  % The purpose of this thesis is to formalize the notion of dissection and its
+  % usage to transform a fold into a tail-recursive function.
+
+  % The first step is to prove that it is possible to write a function that
+  % computes the fold of a non-linear (tree like) structure by tail recursion over
+  % a explicit stack and that this function terminates.
+
+  % This section is devoted to show that by using \emph{well founded} recursion we
+  % can solve the problem for a specific datatype, the binary tree. simplified
+  % version of the problem; that of traversing a tree from left to right. This
+  % simplification from folding to traversing a tree will not be an impediment to
+  % later generalize our results. A traversal can be conceptually thought as a
+  % fold that does nothing.
+
+  % The recursive structure of a inductive type is naturally defined in a top to
+  % bottom manner. However, the traversing function has to exploit the left to
+  % right inductive structure that is implicit in any tree-like type. For this
+  % reason we cannot directly write the function that performs the traversal in
+  % \Agda. The termination checker warns that it does not terminate because the
+  % argument is not --manifestly-- structurally smaller.
+
+  % In \cref{sec:termination} we reviewed several well known techniques that can
+  % be used to assist \Agda's termination checker. \emph{Well founded} recursion
+  % is the only one that allows us to make evident the left to right inductive
+  % structure and provides us with a means for exploiting it.
+
+\subsection{Binary trees}\label{subsec:bintree}
+% Binary tree type
+% Evaluation
+% Abstraction with algebra
+% Catamorphism
+
+  The type of binary trees with natural numbers on the leaves is represented in
+  \Agda using the following inductive type.
+
+\begin{code}
+  data Tree : Set where
+    Tip   :  Nat   -> Tree
+    Node  :  Tree  -> Tree -> Tree
+\end{code}
+
+  As examples of binary trees for example we can have:
+
+  \todo{photo example}
+
+  We can use binary trees to represent the syntax of arithmetic expressions. A
+  value of type |Tree| is an expression where the |Node| constructor stands for
+  addition and the natural numbers stand for themselves. Under this view, we can
+  interpret (or evaluate) an expression into a natural number using a function
+  |eval|.
+
+%{
+%format n     = "\AB{n}"
+%format t1    = "\AB{\ensuremath{t_1}}"
+%format t2    = "\AB{\ensuremath{t_2}}"
+\begin{code}
+  eval : Tree -> Nat
+  eval (Tip n)       = n
+  eval (Node t1 t2)  = eval t1 + eval t2
+\end{code}
+%}
+
+  The function |eval| is defined compositionally (in the style of denotational
+  semantics) where the value of a |Node| is computed by composing the values for
+  the left and right subtree. Analogously, we can have another interpetation
+  function that pretty prints a binary tree. This is a function of type |Tree ->
+  String|.
+
+%{
+%format n     = "\AB{n}"
+%format t1    = "\AB{\ensuremath{t_1}}"
+%format t2    = "\AB{\ensuremath{t_2}}"
+\begin{code}
+  pretty : Tree -> String
+  pretty (Tip n)       = show n
+  pretty (Node t1 t2)  = pretty t1 ++ " + " ++ pretty t2
+\end{code}
+%}
+
+  Both interpretations functions share some underlying structure. In the case of
+  |eval|, when evaluating the constructor |Node| we combine the results of both
+  subtrees using the addition operator |+| while when pretty printing we combine
+  them by concatenating the resulting |String|s.
+
+  Abstracting the concrete functions used in each case into an algebra.
+
+\begin{code}
+  record TreeAlg : Set1 where
+    field
+      A      : Set
+      TipA   : Nat -> A
+      NodeA  : A -> A -> A
+\end{code}
+
+\todo{A has to be in TreeAlg or it should be made parametric over it?}
+
+  We can define a general catamorphism that folds a tree into a value of the
+  type specified by the algebra.
+
+%{
+%format n     = "\AB{n}"
+%format t1    = "\AB{\ensuremath{t_1}}"
+%format t2    = "\AB{\ensuremath{t_2}}"
+\begin{code}
+  treeCata : (tAlg : TreeAlg) → Tree → A tAlg
+  treeCata tAlg (Tip n)       = TipA  tAlg n
+  treeCata tAlg (Node t1 t2)  = NodeA tAlg (treeCata tAlg t1) (treeCata tAlg t2)
+\end{code}
+%}
+
+  Using the catamorphism, the |eval| function can be re-implemented as follows.
+
+%{
+%format tAlg = "\AB{tAlg}"
+\begin{code}
+  eval : Tree -> Nat
+  eval = treeCata tAlg
+    where
+      tAlg : TreeAlg
+      tAlg = record { A = Nat  ;  TipA = id  ;  NodeA = \_+\_ }
+\end{code}
+%}
+
+
+\subsection{Zipper}\label{subsec:zipper}
+
+  Following Huet's idea of a \emph{Zipper}\cite{Huet97thezipper}, any leaf of a
+  binary tree can be represented as a pair of the natural number it holds and
+  the path from the root of the tree to the position it occupies.
+
+\begin{code}
+  UZipper : Set
+  UZipper = Nat * Stack
+\end{code}
+
+  At each |Node| constructor, the path has to record whether the leaf occurs in
+  the left or the right subtree. Moreover, from a value of \emph{Zipper} we
+  should be able to reconstruct the original tree thus each time the path choses
+  between left or right it has to keep track of the remaining subtree.
+
+\begin{code}
+  Stack : Set
+  Stack = List (Tree U+ Tree)
+\end{code}
+
+  In \cref{fig:zipperexample}, there are two examples of \emph{Zipper} where the
+  leaf in focus is marked with a box $\Box$. The \emph{Zipper} shown on the
+  bottom is a tuple with the path to the leaf and the natural number. In the
+  path, a left arrow {\color{red}$\leftarrow$} (correspondingly a right arrow
+  {\color{green}$\rightarrow$}) represents that the rest of the path points to a
+  leaf in the left (right) subtree of the |Node|.
+
+\begin{figure}[h]
+\begin{center}
+  \includegraphics[scale=0.06]{images/zipperexample}
+  \caption{Example of \emph{Zipper}}
+  \label{fig:zipperexample}
+\end{center}
+\end{figure}
+
+  If we were able to freeze a traversal from left to right over a binary tree, a
+  value of type \emph{Zipper} would represent a concrete state of this
+  procedure. At each leaf, everything that has already been traversed appears to
+  the left of the |Stack| while the parts of the tree that still have to be
+  processed show up on the right.
+
+\begin{figure}[h]
+\begin{center}
+  \includegraphics[scale=0.04]{images/zippertraversal}
+  \caption{Example of freezing a traversal}
+  \label{fig:zippertraversal}
+\end{center}
+\end{figure}
+
+  In order to represent the state of folding a binary tree from left to right,
+  we can enrich the type of the |Stack| save not only the left subtrees (in case
+  the path points to the right {\color{green}$\rightarrow$}) but also the value
+  it evaluates (using the catamorphism) to and a proof of this equality.
+
+  The rest of the constructions we are going to show assume there is an ambient
+  tree algebra and that it is constant across all definitions and proofs. To
+  achieve this in \Agda, we create a new module parametrized by a |TreeAlg|.
+
+\begin{code}
+  module _ (tAlg : TreeAlg) where
+
+    open TreeAlg tAlg
+\end{code}
+
+  By |open|ing |tAlg| we bring into scope the type |A| and the fields |TipA| and
+  |NodeA| without need to make any further reference to |tAlg|. The type of
+  |Stack| is now defined as follows.
+
+%{
+%format a  = "\AB{a}"
+%format t  = "\AB{t}"
+%format eq = "\AB{eq}"
+
+\begin{code}
+  Stack : Set
+  Stack = List (Tree U+ Sigma A lambda a  -> Sigma Tree lambda t
+                                          -> treeCata tAlg t == a)
+
+  pattern Left   t       = inj1 t
+  pattern Right  a t eq  = inj2 (a , t , eq)
+\end{code}
+
+  The only piece of information required to compute the catamorphism of a |Tree|
+  are the |a| values that come from evaluating the subtrees that appear to the
+  left of the position under focus. However, as we will show later in
+  \todo{ref}, it is neccesary for proving termination to keep around the |Tree|
+  where the value came from. We say that |t| and the equality proof in
+  |Stack| are computationally irrelevant. However, in \Agda~we cannot express
+  such fact\footnote{In other systems like Coq the Tree would live in Prop}.
+%}
+
+  Given a |Stack| and a |Tree| (we can always embed a |Nat| into a |Tree| using
+  |Tip|), the original |Tree| can be reconstructed by recursing over the
+  |Stack|. At each step, it is known to which subtree the position belongs.
+
+%{
+%format t  = "\AB{t}"
+%format t1 = "\AB{t\ensuremath{_1}}"
+%format s  = "\AB{s}"
+\begin{code}
+    plugD : Tree → Stack → Tree
+    plugD t []                  = t
+    plugD t (Left t1 :: s)       = Node (plugD t s) t1
+    plugD t (Right _ t1 _ :: s)  = Node t1 (plugD t s)
+\end{code}
+
+  Until now, we have only considered that the |Stack| represents the path from
+  the root of the tree way down to the focused leaf. We can instead reverse the
+  |Stack| part of the \emph{Zipper} so the path travels bottom-up from the leaf
+  up to the root of the tree.
+
+\begin{figure}[h]
+\begin{center}
+  \includegraphics[scale=0.05,angle=270]{images/zipperbuvstd}
+  \caption{Bottom-Up versus Top-Down \emph{Zipper}}
+  \label{fig:zipperbuvstd}
+\end{center}
+\end{figure}
+
+  Under this view, we can reconstruct the original |Tree| from the
+  |Stack|.
+
+\begin{code}
+  plugU : Tree -> Stack -> Tree
+  plugU t (Left   t1 :: s)      = plugU (Node t t1) s
+  plugU t (Right  _ t1 _ :: s)  = plugU (Node t1 t) s
+  plugU t []                   = t
+\end{code}
+%}
+
+  The only difference between both interpretations of the \emph{Zipper} is that
+  to translate from one to the other we just need to reverse the |Stack|. We can
+  show that indeed the original |Tree| is preserved by the conversion.
+
+%{
+%format plugU-to-plugD = plugU "\AF{-to-}" plugD
+%format plugD-to-plugU = plugD "\AF{-to-}" plugU
+%format reverse = "\AF{reverse}"
+%format t = "\AB{t}"
+%format s = "\AB{s}"
+%format z = "\AB{z}"
+
+\begin{code}
+    plugU-to-plugD : forall t s -> plugU t s == plugD t (reverse s)
+    plugU-to-plugD  t  s = cdots
+
+    plugD-to-plugU : forall t s -> plugD t s == plugU t (reverse s)
+    plugD-to-plugU t  s = cdots
+\end{code}
+
+\subsection{One-step of a fold}\label{subsec:onestep}
+
+  The \emph{Zipper} type represents a snapshot of the internal state of a
+  catamorphism over a binary tree. From one value of \emph{Zipper} we can write
+  a pair of functions, |load| and |unload| that combined together perform one
+  step of the fold.
+
+\begin{code}
+    load : Tree -> Stack -> UZipper U+ A
+    load (Tip x) s       = inj1 (x , s)
+    load (Node t₁ t₂) s  = load t₁ (Left t₂ ∷ s)
+
+    unload : (t : Tree) → (a : A) → (eq : treeCata tAlg t) ≡ a -> Stack -> UZipper U+ A
+    unload t a eq []                     = inj2 a
+    unload t a eq (Left t′ ∷ s)          = load t′ (Right a t eq :: s)
+    unload t a eq (Right a′ t′ eq′ ∷ s)  = unload  (Node t′ t) (NodeA a′ a) (cong₂ NodeA eq′ eq) s
+\end{code}
+
+  The function |unload| traverses the |Stack| combining all the results of
+  evaluating the subtrees that were on the left of the position until either
+  reaches a |Node| that has an unevaluated subtree on the right (|Left|
+  constructor) or the |Stack| is empty and the |Tree| has been fully evaluated.
+  When the former case occurs the |load| function is in charge of traversing the
+  subtree on the right to find the leftmost leaf.
+
+  \todo{maybe talk about irrelevance of t and eq?}
+
+  A folding step just consists of calling |unload| passing appropiate arguments.
+
+\begin{code}
+    step : UZipper -> UZipper U+ A
+    step (n , s) = unload (Tip n) (TipA n) refl s
+\end{code}
+
+  More graphically, the proccess of folding the tree one step is depicted in in
+  \cref{fig:onestep},
+
+\begin{figure}[h]
+\begin{center}
+  \includegraphics[scale=0.05,angle=180]{images/onestep}
+  \caption{One step of fold}
+  \label{fig:onestep}
+\end{center}
+\end{figure}
+%}
+
+\subsection{Folding a |Tree|}
+
+  From the machinery we have developed so far one would be inclined to think
+  that in order to fold a |Tree| it will suffice to find a fixed point of the
+  function |step|.
+
+\begin{code}
+  foldTree : Tree -> Nat
+  foldTree t with load t []
+  ... | inj2 n = n
+  ... | inj1 z = rec z
+    where
+      rec : UZipper -> Nat
+      rec z with step z
+      ... | inj1 z'  = rec z'
+      ... | inj2 n   = n
+\end{code}
+
+  However, it does not work. \Agda's termination checker is right when it warns
+  that the |z'| passed as an argument to the recursive call on |rec| is not
+  structurally smaller than |z| and therefore the fixed point of |step| might
+  not exists\footnote{|rec| loops forever}.
+
+  From an outer perspective, it is fair to assert that for any possible input of
+  type |UZipper|, the function |rec| has a fixed point. A value of |UZipper|
+  focus on the position of a concrete leaf in a value of type |Tree|, and the
+  function |step| refocuses the to the next leaf on the right. Because there are
+  finitely many leaves on a |Tree|, the function |rec| must always terminate.
+
+  In order to solve this problem, in the next subsections we will develop the
+  notion of indexed \emph{Zipper} and show how it allows us to define an order
+  relation between positions (\emph{Zipper}s) of the same |Tree|. This will be
+  the key to define |rec| by structural recursion.
+
+\subsection{Indexed \emph{Zipper}}\label{subsec:ixzipper}
+
+  The current type of \emph{Zipper}, |UZipper| does not encode too much
+  information. Given a value, it is not possible to statically know the |Tree|
+  from which it represents a position. If we are to compare a pair of |UZipper|
+  we need them to represent positions on the same |Tree| otherwise it does not
+  make sense.
+
+  We can address this shortcoming in the current representation by creating a
+  new type wrapper over |UZipper| that is type indexed by the |Tree| where it is
+  a position.
+
+\begin{code}
+  plugZD : UZipper -> Tree
+  plugZD (t , s) = plugD (Tip t) s
+\end{code}
+
+\begin{code}
+  data ZipperD (t : Tree) : Set where
+    _,_ : (z : UZipper) -> plugZD z == t -> ZipperD t
+\end{code}
+
+  From an indexed \emph{Zipper} we can forget the extra information and recover
+  the original |UZipper|.
+
+\begin{code}
+    forgetD : ∀ {t : Tree} -> (z : ZipperD t) -> UZipper
+    forgetD (z , _) = z
+\end{code}
+%}
+\subsection{\emph{Well founded} recursion}
+
+\subsection{Catamorphism}
+\subsection{Correctness}
+\subsection{Discussion}
+
+%   Any tree-like datatype shares a common branching structure with the type of
+%   skeleton binary trees. We will use this type as the basis of our work.
+
+%   \InsertCode{Proposal/Tree/Base.tex}{Tree}
+
+%   Following Huet's idea of a \emph{Zipper}\cite{Huet97thezipper}, any position
+%   in the tree can be represented as a pair of a subtree and a stack that holds
+%   all the trees, to the left and to the right, in the path to the root.
+
+%   \InsertCode{Proposal/Tree/Base.tex}{Stack}
+
+%   Given a value of type \AD{Zipper} it is possible to \emph{plug} the subtree
+%   and the stack together to reconstruct the original tree.
+
+%   \InsertCode{Proposal/Tree/Base.tex}{BUPlug}
+
+%   Navigating one position to the right in the tree can be easily defined in a
+%   tail-recursive manner.
+
+%   \InsertCode{Proposal/Tree/Base.tex}{BURight}
+
+%   However, it is not possible to write a function that calculates the rightmost
+%   position of the tree by iterating the \AF{right} function until it yields
+%   \AI{nothing}.
+
+%   \InsertCode{Proposal/Tree/Base.tex}{BUIterate}
+
+%   Pattern matching on the result of \AF{right}\AS{}\AB{z} does not reveal any
+%   structural relation between the input \AB{z} and \AB{z₁}. Thus \Agda~'s
+%   termination checker rightfully classifies the function as non-terminating. It
+%   does not know in which sense the recursive call is made on a smaller argument.
+
+% \subsection{Setting the stage}
+% \label{subsec:preparing}
+
+%   To be able to define \AF{rightmost}, we should find the structure
+%   that decreases with each call to the function \AF{right} so \AF{rightmost} can
+%   be defined by \emph{well founded} recursion over it.
+
+%   Any position in the tree has a finite number of positions to the right of
+%   itself. A value of type \AD{Zipper} represents a position in the tree and for
+%   this reason each time we apply the function \AF{right} to some input the
+%   number of positions to the right decreases.
+
+%   Using \emph{well founded} recursion, as explained in \cref{sec:termination},
+%   we can define a relation \AD{\_<\_} over elements of \AD{Zipper} that exposes
+%   the decreasing structure of moving to the right.
+
+%   Additionally, by proving \textit{well foundedness} of the relation and the
+%   property that whenever the evaluation of \AF{right} \AB{z} yields a
+%   \AI{just}\AS{}\AB{z₁} then \mbox{\AB{z₁}\AS{}\AD{<}\AS{}\AB{z}}, we will be
+%   able to define \AF{rightmost} by structural recursion on the accessibility
+%   predicate of \AD{\_<\_}.
+
+%   \InsertCode{Proposal/Tree/Base.tex}{Skeleton}
+
+%   The purpose of the following subsections is to show how we can fill
+%   the open holes and the definition of \AD{\_<\_}.
+
+% \subsection{Defining the relation}
+
+%   The relation we need shall consider positions on the left subtree of a
+%   \AI{Node} bigger than the \AI{Node} itself which at the same time is bigger
+%   than any position in its right subtree.
+
+%   Following Huet's idea, we regard the \AD{Stack} type as a path going
+%   \textit{backwards} from the position of the subtree up to the root. The
+%   relation has to be inductively defined on the \AD{Stack} part of the
+%   \AD{Zipper}.  Removing a constructor from the \AD{Stack} means moving up a
+%   position on the tree.
+
+%   For any two arbitrary positions on the tree, it is unknown a priori what is
+%   the order of removing constructors from the stack, that has to be followed to
+%   reach one of the base cases.
+%   Because of this, the relation has to be able to handle all possible situations
+%   which effectively will lead to a relation that allows us to prove that any two
+%   elements are related in both directions. Needless to say that such relation
+%   is just useless for our mission: a change of representation is needed.
+
+%   As an alternative, we can consider the \AD{Stack} as the \textit{forward} path
+%   from the root to the position where the subtree is located. A \emph{plug} operator
+%   that reconstruct the tree from the root can also be defined.
+
+%   \InsertCode{Proposal/Tree/Base.tex}{TDPlug}
+
+%   The new representation for positions is better suited for defining the
+%   relation where positions to the right are considered smaller than positions to
+%   the left. However, for our purpose of traversing the tree tail recursively,
+%   the \textit{backward} representation is a more natural fit.
+
+%   For this reason it is convenient to keep both representations and have a means
+%   of converting from one to the other. The conversion amounts to reverse the
+%   \AD{Stack}. To be sure that both representations are equivalent we can prove
+%   that plugging in one should yield the same tree as converting and plugging in
+%   the other.
+
+%   \InsertCode{Proposal/Tree/Base.tex}{Convert}
+
+%   We are ready to define the relation between elements of type \AD{Zipper}. The
+%   main idea of the relation is to look in the \AD{Stack} part of the \AD{Zipper}
+%   for the point where both \AD{Stack}s diverge.
+
+%   Once this happens, the \AD{Stack} that has a \AI{Left} constructor on top
+%   indicates that its position is located in the left subtree of the \AI{Node} and
+%   therefore should be always considered smaller than the \AI{Node} itself and
+%   than any position that is in the right subtree.
+
+%   When the topmost constructor of the \AD{Stack} is \AI{Right} this means that
+%   the location is in the right subtree. This position is smaller than the
+%   \AI{Node} itself and any other position on the left subtree.
+
+%   The relation we defined is formalized in \Agda~as follows.
+
+%   \InsertCode{Proposal/Tree/Base.tex}{TDRel}
+
+%   Two values of type \AD{Zipper} related by \AD{\_<\_} should represent
+%   positions in the same tree. By including the information of how the subtrees
+%   are reconstructed from the \AD{Tree} and \AD{Stack} on the other side of the
+%   relation this invariant is enforced in the type level.
+%   We can indeed prove that any two related elements when \emph{plugged} yield
+%   the same tree.
+
+%   \InsertCode{Proposal/Tree/Base.tex}{Related}
+
+% \subsection{Proving \textit{well foundedness}}
+
+%   The relation itself would be useless if we cannot prove that it is \emph{well
+%   founded}. As it was explained in \cref{subsec:wf}, the \emph{well foundedness}
+%   property for a relation requires us to exploit the recursive structure of either
+%   the input, in the base cases, or the proof, in the inductive cases. If
+%   we are not able to show \Agda's termination checker that the argument is
+%   --obviously-- structurally smaller then we would not be able to use recursion
+%   to prove \emph{well foundedness}.
+
+%   The naive approach to the proof fails because in general pattern matching on
+%   the \AD{\_<\_} proof does not reveal any information about the structure of
+%   the tree of which the two \AD{Zipper}s are a decomposition.
+
+%   In the base cases, the structure we need to perform recursion is exactly the
+%   subtrees of the original tree, however this is not explicit in the proof.
+
+%   This realisation motivates us to define a new relation over \AD{Zipper} that
+%   makes the tree explicit. Even though we proved that related \AD{Zipper} values
+%   are positions of the same tree we include the proofs that both trees
+%   reconstruct to the same tree in the relation so during the proof we can refine
+%   the structure of the tree by pattern matching. This is the crucial step that
+%   allows the proof of \emph{well foundedness} to succeed.
+
+%   \InsertCode{Proposal/Tree/Base.tex}{TDRelIx}
+
+%   Because the new relation is indexed by a \AD{Tree} the definition of what it
+%   means for this relation to be \emph{well founded} has to change accordingly. The
+%   relation is \emph{well founded} if for any \AD{Tree} any position of it,
+%   \AD{Zipper}, is accessible.
+
+%   \InsertCode{Proposal/Tree/Base.tex}{WF}
+
+%   The full proof is omitted but can be found in the accompanying code. It works
+%   by induction on the \AD{\_<\_} structure as before, but it uses the equality
+%   proofs to discover the smaller structure on which perform recursion.
+
+% \subsection{Navigating through the tree}
+
+%   Finally we have developed the necessary machinery to fill the holes of the
+%   program we proposed in \cref{subsec:preparing}. The definition of \AF{rightmost}
+%   is more complex than we originally devised due to the change of representation
+%   that we use. Moreover, the full proof that \AF{right} yields a smaller element
+%   involves a lot of auxiliary lemmas and a lot of rewriting regarding the
+%   properties of list concatenation and reversal.
+
+%   \InsertCode{Proposal/Tree/Base.tex}{Right-preserves}
+%   \vspace*{-0.5cm}
+%   \InsertCode{Proposal/Tree/Base.tex}{to-right}
+%   \vspace*{-0.5cm}
+%   \InsertCode{Proposal/Tree/Base.tex}{Rightmost}
+
+% \subsection{From traverse to fold}\label{subsec:traverse-to-fold}
+
+%   Once we have shown how it is possible to prove in \Agda~ that the traversal of
+%   a tree from left to right in a tail recursive fashion terminates we are ready
+%   to extend the work to show that the tail recursive counterpart of a fold also
+%   terminates.
+
+%   In this subsection we build the basis for the work on the thesis that will
+%   allow us to prove the termination of a tail recursive fold. As a more interesting
+%   example we will use the type of binary trees with natural numbers in the
+%   leaves which resemble arithmetic expressions.
+
+%   \InsertCode{Proposal/Tree/Fold.tex}{Tree}
+
+%   The fold requires that the stack records both the subtrees that still need to
+%   be traversed and the intermediate results that have not yet been consumed.  For
+%   this reason, the \AD{Stack} datatype now becomes:
+
+%   \InsertCode{Proposal/Tree/Fold.tex}{Stack}
+
+%   In the case of the trees we are using, we can define an analogous
+%   \emph{plugging} operator for both the \textit{backwards} and \textit{forwards}
+%   view of the \AD{Stack}. Because the \AD{Stack} does not represent a path on
+%   the original tree but is just a partial image of how the evaluation proceeds, we
+%   embed the intermediate results as leaves to be able to output a full tree.
+
+%   \InsertCode{Proposal/Tree/Fold.tex}{Plug}
+
+%   As opposed to McBride's example as explained in \cref{subsec:problem} we
+%   will not consider the tail recursive version of a fold as a pair of functions,
+%   \AF{load} and \AF{unload}. Instead we will define a function that performs
+%   only one step of the computation at a time. This will be needed to prove that
+%   each step of the computation decreases regarding the relation thus it is
+%   possible to define the tail recursive fold using \emph{well founded} recursion.
+
+%   \InsertCode{Proposal/Tree/Fold.tex}{load-unload}
+
+%   If we define a suitable relation over \AD{Zipper} we should be able to define
+%   fold by iterating \AF{load/unload} until it yields a natural number.
+
+%   \InsertCode{Proposal/Tree/Fold.tex}{fold}
+
+%   The relation is not as straightforward to define as it was in the case of
+%   traversing the tree with a \AD{Zipper} because now the structure of the tree
+%   changes during the folding process.
+
+%   Two related elements by \AD{\_<\_} need not to reconstruct to the same tree
+%   but instead they reconstruct to a \textbf{partial image} of the original tree
+%   where some full subtrees have been replaced by the values they denote.
